RGA as set - wip

inductive_proof/RGA_set_pre-cond/App_do_pre_first.fst
@@ -62,8 +62,8 @@ let do_pre (s:concrete_st) (op:op_t) : prop =
 
 let do_prop (s:concrete_st) (op:op_t) :
   Lemma (ensures (Add_after? (snd op) ==> (do_pre s op <==>
-                           ~ (mem_id_s (fst op) (fst s)))) /\ //get_after_id op <> fst op /\                          
-                                  //(~ ((get_after_id op) = 0) ==> mem_id_s (get_after_id op) (fst s)))) /\
+                           ~ (mem_id_s (fst op) (fst s)) /\ //get_after_id op <> fst op /\                          
+                                  (~ ((get_after_id op) = 0) ==> mem_id_s (get_after_id op) (fst s)))) /\
                  (Remove? (snd op) ==> (do_pre s op <==>
                           mem_id_s (get_rem_id op) (fst s)))) = ()
 
@@ -73,8 +73,7 @@ let do (s:concrete_st) (op:op_t{do_pre s op})
                    //(Remove? (snd op) ==> (forall id. S.mem id (snd r) <==> S.mem id (snd s) \/ id = get_rem_id op)) /\*)
                     S.subset (fst s) (fst r) /\ S.subset (snd s) (snd r)}) =
    match op with
-  |(ts, Add_after after_id ele) -> //if after_id <> 0 && not (mem_id_s after_id (fst s)) then s else
-                                   (S.add (ts, (after_id, ele)) (fst s), snd s)
+  |(ts, Add_after after_id ele) -> (S.add (ts, (after_id, ele)) (fst s), snd s)
   |(_, Remove id) -> (fst s, S.add id (snd s))
   
 let lem_do (a b:concrete_st) (op:op_t)
@@ -136,6 +135,93 @@ let linearizable_s2_0' (lca s1 s2:st)
                     merge_pre (v_of lca) (v_of s1) (v_of s2))
           (ensures eq (v_of s1) (concrete_merge (v_of lca) (v_of s1) (v_of s2))) = ()
 
+let rec lem_foldl (s:concrete_st) (l:log)
+  : Lemma (requires do_pre_prop s l)
+    (ensures (length l > 0 ==> (S.subset (fst s) (fst (apply_log s l))) /\
+                              (S.subset (snd s) (snd (apply_log s l)))))
+          (decreases length l)
+  = match length l with
+    |0 -> ()
+    |_ -> lem_foldl (do s (head l)) (tail l)
+
+#push-options "--z3rlimit 100" 
+let merge_pre_prop (lca s1 s2:st) (last1 last2:op_t)
+  : Lemma (requires do_pre (v_of s1) last1 /\ do_pre (v_of s2) last2 /\ 
+                    consistent_branches lca (do_st s1 last1) (do_st s2 last2) /\
+                    consistent_branches lca s1 s2 /\
+                    fst last1 <> fst last2 /\
+                    merge_pre (v_of lca) (do (v_of s1) last1) (do (v_of s2) last2))
+          (ensures merge_pre (v_of lca) (v_of s1) (do (v_of s2) last2) /\
+                   merge_pre (v_of lca) (do (v_of s1) last1) (v_of s2)) =
+  split_prefix init_st (ops_of lca) (ops_of s1);
+  lem_foldl (v_of lca) (diff (ops_of s1) (ops_of lca));
+  split_prefix init_st (ops_of lca) (ops_of s2);
+  lem_foldl (v_of lca) (diff (ops_of s2) (ops_of lca))
+  (*assert (forall id. mem_id_s id (fst (v_of lca)) ==> ~ (mem_id_s id (S.difference (fst (v_of s1)) (fst (v_of lca)))));
+  assert (forall id. mem_id_s id (fst (v_of lca)) ==> ~ (mem_id_s id (S.difference (fst (v_of s2)) (fst (v_of lca)))));
+  assert (forall id. mem_id_s id (S.difference (fst (v_of s1)) (fst (v_of lca))) ==> 
+                ~ (mem_id_s id (S.difference (fst (do (v_of s2) last2)) (fst (v_of lca)))));
+  assert (forall id. mem_id_s id (S.difference (fst (do (v_of s1) last1)) (fst (v_of lca))) ==> 
+                ~ (mem_id_s id (S.difference (fst (v_of s2)) (fst (v_of lca)))));
+  ()*)
+
+let lem_cond (lca s1 s2:st) (last1 last2:op_t)
+  : Lemma (requires do_pre (v_of s1) last1 /\ do_pre (v_of s2) last2 /\ 
+                    consistent_branches lca (do_st s1 last1) (do_st s2 last2) /\
+                    consistent_branches lca s1 s2 /\
+                    fst last1 <> fst last2 /\
+                    merge_pre (v_of lca) (do (v_of s1) last1) (do (v_of s2) last2) /\
+                    merge_pre (v_of lca) (do (v_of s1) last1) (v_of s2) /\
+                    merge_pre (v_of lca) (v_of s1) (do (v_of s2) last2))
+          (ensures (Add_after? (snd last1) /\ Add_after? (snd last2) ==>
+                      fst last1 <> get_after_id last2 /\ fst last2 <> get_after_id last1) /\
+                   (Remove? (snd last1) /\ Add_after? (snd last2) ==> fst last2 <> get_rem_id last1) /\
+                   (Remove? (snd last2) /\ Add_after? (snd last1) ==> fst last1 <> get_rem_id last2)) = ()
+
+#push-options "--z3rlimit 200" 
+let linearizable_gt0_s1' (lca s1 s2:st) (last1 last2:op_t)
+  : Lemma (requires do_pre (v_of s1) last1 /\ do_pre (v_of s2) last2 /\ 
+                    consistent_branches lca (do_st s1 last1) (do_st s2 last2) /\
+                    consistent_branches lca s1 (do_st s2 last2) /\
+                    consistent_branches lca s1 s2 /\
+                    is_prefix (ops_of lca) (ops_of s2) /\
+                    fst last1 <> fst last2 /\
+                    First_then_second? (resolve_conflict last1 last2) /\
+                    merge_pre (v_of lca) (do (v_of s1) last1) (do (v_of s2) last2))
+          (ensures merge_pre (v_of lca) (v_of s1) (do (v_of s2) last2) /\
+                   do_pre (concrete_merge (v_of lca) (v_of s1) (do (v_of s2) last2)) last1 /\
+                   eq (do (concrete_merge (v_of lca) (v_of s1) (do (v_of s2) last2)) last1)
+                      (concrete_merge (v_of lca) (do (v_of s1) last1) (do (v_of s2) last2))) = 
+  resolve_conflict_prop last1 last2;
+  merge_pre_prop lca s1 s2 last1 last2;
+  lem_cond lca s1 s2 last1 last2
+
+let linearizable_gt0_s2' (lca s1 s2:st) (last1 last2:op_t)
+  : Lemma (requires do_pre (v_of s1) last1 /\ do_pre (v_of s2) last2 /\ 
+                    consistent_branches lca (do_st s1 last1) (do_st s2 last2) /\
+                    consistent_branches lca (do_st s1 last1) s2 /\
+                    consistent_branches lca s1 s2 /\
+                    is_prefix (ops_of lca) (ops_of s1) /\
+                    fst last1 <> fst last2 /\
+                    Second_then_first? (resolve_conflict last1 last2) /\
+                    merge_pre (v_of lca) (do (v_of s1) last1) (do (v_of s2) last2)) 
+          (ensures merge_pre (v_of lca) (do (v_of s1) last1) (v_of s2) /\
+                   do_pre (concrete_merge (v_of lca) (do (v_of s1) last1) (v_of s2)) last2 /\
+                   eq (do (concrete_merge (v_of lca) (do (v_of s1) last1) (v_of s2)) last2)
+                      (concrete_merge (v_of lca) (do (v_of s1) last1) (do (v_of s2) last2))) = 
+  resolve_conflict_prop last1 last2;
+  merge_pre_prop lca s1 s2 last1 last2;
+  lem_cond lca s1 s2 last1 last2
+
+/////////////////////////////////////////////////////////////////////////////////
+
+
+
+
+/////////////////////////////////////////////////////////////////////////////////
+
+
+
 let pre1_pre2_s2 (lca s1 s2:st)
     : Lemma (requires consistent_branches_s2_gt0 lca s1 s2)
             (ensures consistent_branches lca s1 (inverse_st s2)) = 
@@ -150,54 +236,49 @@ let pre1_pre2_s1 (lca s1 s2:st)
   lastop_diff (ops_of lca) (ops_of s1);
   inverse_diff_id_s1' (ops_of lca) (ops_of s1) (ops_of s2)
   
-#push-options "--z3rlimit 600" 
+#push-options "--z3rlimit 400" 
 let rec invalid_exec1 (lca s1 s2:st) (last1 last2:op_t)
   : Lemma (requires do_pre (v_of s1) last1 /\ do_pre (v_of s2) last2 /\ 
                     consistent_branches lca (do_st s1 last1) (do_st s2 last2) /\
                     consistent_branches lca s1 s2 /\
                     Add_after? (snd last1) /\ Remove? (snd last2) /\
                     fst last1 <> fst last2)
-          (ensures (fst last1 <> get_rem_id last2) (*/\
-                   (Remove? (snd last1) /\ Add_after? (snd last2) ==> fst last2 <> get_rem_id last1) /\
-                   (Add_after? (snd last1) /\ Add_after? (snd last2) ==>
-                      fst last1 <> get_after_id last2 /\ fst last2 <> get_after_id last1*))
+          (ensures (fst last1 <> get_rem_id last2))
           (decreases %[length (ops_of s1); length (ops_of s2)]) = 
-  //assume ((fst last1 = get_rem_id last2) ==> ~ (Add_after? (snd last1) /\ Remove? (snd last2)));
   if ops_of lca = ops_of s1 then
-    (if ops_of lca = ops_of s2 then admit()
+    (if ops_of lca = ops_of s2 then ()
      else 
        (let s2' = inverse_st s2 in
         let pre2, lastop2 = un_snoc (ops_of s2) in
-        do_prop (v_of s2') last2; //include it if needed
+        do_prop (v_of s2') last2; 
         lem_apply_log init_st (ops_of s2);
         inverse_helper init_st pre2 lastop2;
-        assume (mem_id_s (get_rem_id last2) (fst (v_of s2')) <==> do_pre (v_of s2') last2);
+        assert (mem_id_s (get_rem_id last2) (fst (v_of s2')) <==> do_pre (v_of s2') last2);
         pre1_pre2_s2 lca s1 s2;
         if mem_id_s (get_rem_id last2) (fst (v_of s2')) then 
-          (admit();assume (do_pre (v_of s2') last2); 
+          (assert(do_pre (v_of s2') last2); 
            assume (consistent_branches lca (do_st s1 last1) (do_st s2' last2)); //can be done
            invalid_exec1 lca s1 s2' last1 last2)
         else 
-          (assume (not (mem_id_s (get_rem_id last2) (fst (v_of s2'))));
+          (assert (not (mem_id_s (get_rem_id last2) (fst (v_of s2'))));
            if Add_after? (snd lastop2) && fst lastop2 = get_rem_id last2 then 
              (lem_diff (snoc (ops_of s2) last2) (ops_of lca);
               lem_diff (ops_of s2) (ops_of lca); 
-              assume (mem_id (fst lastop2) (diff (ops_of s2) (ops_of lca)));
-              assume (not (mem_id (fst lastop2) (ops_of lca)));
-              assume (mem_id (fst lastop2) (ops_of s2));
+              assert (mem_id (fst lastop2) (diff (ops_of s2) (ops_of lca)));
+              assert (not (mem_id (fst lastop2) (ops_of lca)));
+              assert (mem_id (fst lastop2) (ops_of s2));
               lemma_append_count_assoc_fst (ops_of s2) (create 1 last2);
-              assume (mem_id (fst lastop2) (snoc (ops_of s2) last2)); 
-              lemma_append_count_assoc_fst (snoc (ops_of s2) last2) (create 1 last2);
-              assume (mem_id (fst lastop2) (diff (snoc (ops_of s2) last2) (ops_of lca)));
+              assert (mem_id (fst lastop2) (snoc (ops_of s2) last2)); 
+              assert (mem_id (fst lastop2) (diff (snoc (ops_of s2) last2) (ops_of lca)));
               lem_diff (snoc (ops_of s1) last1) (ops_of lca);
-              assume (mem_id (fst last1) (diff (snoc (ops_of s1) last1) (ops_of lca))); //done
+              assert (mem_id (fst last1) (diff (snoc (ops_of s1) last1) (ops_of lca))); 
               ()) 
            else 
-             (admit();assume (do_pre (v_of s2') last2); 
+             (assert (do_pre (v_of s2') last2); 
               assume (consistent_branches lca (do_st s1 last1) (do_st s2' last2)); //can be done
               invalid_exec1 lca s1 s2' last1 last2))))
   else 
-    (admit()(*;let s1' = inverse_st s1 in 
+    (let s1' = inverse_st s1 in 
      assume (consistent_branches_s1_gt0 lca s1 s2);
      let pre1, lastop1 = un_snoc (ops_of s1) in
      do_prop (v_of s1') last1; //include it if needed
@@ -206,23 +287,144 @@ let rec invalid_exec1 (lca s1 s2:st) (last1 last2:op_t)
      pre1_pre2_s1 lca s1 s2;
      assume (fst lastop1 <> fst last1); //can be done
      if Add_after? (snd lastop1) && fst lastop1 <> get_after_id last1 then 
-       (admit();assume (not (mem_id_s (fst last1) (fst (v_of s1'))));
-        //assume (~ (get_after_id last1 = 0) ==> mem_id_s (get_after_id last1) (fst (v_of s1')));
-        assume (do_pre (v_of s1') last1);
+       (assert (not (mem_id_s (fst last1) (fst (v_of s1'))));
+        assert (do_pre (v_of s1') last1);
         assume (consistent_branches lca (do_st s1' last1) (do_st s2 last2)); //can be done
         invalid_exec1 lca s1' s2 last1 last2)
      else if Add_after? (snd lastop1) && fst lastop1 = get_after_id last1 then  //check this case with full do_pre for add
-       (admit();assume (not (mem_id_s (fst last1) (fst (v_of s1')))); 
-        //assert (~ (get_after_id last1 = 0) ==> mem_id_s (get_after_id last1) (fst (v_of s1')));
-        assume (do_pre (v_of s1') last1);
-        assume (consistent_branches lca (do_st s1' last1) (do_st s2 last2)); //can be done
-        invalid_exec1 lca s1' s2 last1 last2)
+       admit()
      else if Remove? (snd lastop1) && get_rem_id lastop1 <> fst last1 then
-       (admit();assume (do_pre (v_of s1') last1); 
+       (assert (do_pre (v_of s1') last1); 
         assume (consistent_branches lca (do_st s1' last1) (do_st s2 last2)); //can be done
         invalid_exec1 lca s1' s2 last1 last2)
-     else admit()*)) //Remove? (snd lastop1) && get_rem_id lastop1 = fst last1
+     else ()) //Remove? (snd lastop1) && get_rem_id lastop1 = fst last1
 
+
+let rec invalid_exec2 (lca s1 s2:st) (last1 last2:op_t)
+  : Lemma (requires do_pre (v_of s1) last1 /\ do_pre (v_of s2) last2 /\ 
+                    consistent_branches lca (do_st s1 last1) (do_st s2 last2) /\
+                    consistent_branches lca s1 s2 /\
+                    Add_after? (snd last1) /\ Add_after? (snd last2) /\
+                    fst last1 <> fst last2 /\
+                    merge_pre (v_of lca) (do (v_of s1) last1) (do (v_of s2) last2) /\
+                    merge_pre (v_of lca) (v_of s1) (do (v_of s2) last2) /\
+                    merge_pre (v_of lca) (do (v_of s1) last1) (v_of s2))
+          (ensures fst last1 <> get_after_id last2 (* /\ fst last2 <> get_after_id last1*))
+          (decreases %[length (ops_of s1); length (ops_of s2)]) = 
+  if ops_of lca = ops_of s1 then
+    (if ops_of lca = ops_of s2 then () //done
+     else 
+       (let s2' = inverse_st s2 in
+        let pre2, lastop2 = un_snoc (ops_of s2) in
+        do_prop (v_of s2') last2; //include it if needed
+        lem_apply_log init_st (ops_of s2);
+        inverse_helper init_st pre2 lastop2;
+        pre1_pre2_s2 lca s1 s2;
+        assume (fst lastop2 <> fst last2); //can be done
+        if Remove? (snd lastop2) then
+          (assert (do_pre (v_of s2') last2); 
+           pre1_pre2_s2 lca s1 s2;
+           assume (consistent_branches lca (do_st s1 last1) (do_st s2' last2)); //can be done
+           invalid_exec2 lca s1 s2' last1 last2)
+        else if Add_after? (snd lastop2) && fst lastop2 <> get_after_id last2 then
+          (assert (do_pre (v_of s2') last2); //done
+           pre1_pre2_s2 lca s1 s2;
+           assume (consistent_branches lca (do_st s1 last1) (do_st s2' last2)); //can be done
+           invalid_exec2 lca s1 s2' last1 last2)
+        else 
+          (lem_diff (snoc (ops_of s2) last2) (ops_of lca);
+           lem_diff (ops_of s2) (ops_of lca); 
+           lemma_append_count_assoc_fst (ops_of s2) (create 1 last2);
+           assert (mem_id (fst lastop2) (diff (snoc (ops_of s2) last2) (ops_of lca)));
+           lemma_mem_append (ops_of s1) (create 1 last1);
+           assert (snoc (ops_of s1) last1 == Seq.append (ops_of s1) (create 1 last1));
+           lemma_append_count_assoc_fst (ops_of s1) (create 1 last1);
+           assert (mem_id (fst last1) (snoc (ops_of s1) last1));
+           lem_diff (snoc (ops_of s1) last1) (ops_of lca);
+           assert (mem_id (fst last1) (diff (snoc (ops_of s1) last1) (ops_of lca)));
+           ())))
+  else 
+    (let s1' = inverse_st s1 in 
+     assert (consistent_branches_s1_gt0 lca s1 s2);
+     let pre1, lastop1 = un_snoc (ops_of s1) in
+     do_prop (v_of s1') last1; //include it if needed
+     lem_apply_log init_st (ops_of s1);
+     inverse_helper init_st pre1 lastop1;
+     pre1_pre2_s1 lca s1 s2;
+     assume (fst lastop1 <> fst last1); //can be done
+     if Remove? (snd lastop1) then 
+       (assert (do_pre (v_of s1') last1); //done
+        assume (consistent_branches lca (do_st s1' last1) (do_st s2 last2)); //can be done
+        invalid_exec2 lca s1' s2 last1 last2)
+     else if Add_after? (snd lastop1) && fst lastop1 <> get_after_id last1 then 
+       (assert (do_pre (v_of s1') last1); //done
+        assume (consistent_branches lca (do_st s1' last1) (do_st s2 last2)); //can be done
+        invalid_exec2 lca s1' s2 last1 last2)
+     else 
+       admit())
+
+///////////////////////////////////////////////////////////////////
+
+
+
+(*let merge_prop (lca s1:st) (last1:op_t)
+  : Lemma (requires do_pre (v_of s1) last1 /\
+                    distinct_ops (ops_of lca) /\ distinct_ops (ops_of s1) /\
+                    distinct_ops (snoc (ops_of s1) last1) /\
+                    is_prefix (ops_of lca) (ops_of s1) /\ 
+                    is_prefix (ops_of lca) (snoc (ops_of s1) last1) /\ 
+                    (forall id id1. mem_id id (ops_of lca) /\ mem_id id1 (diff (ops_of s1) (ops_of lca)) ==> lt id id1) /\
+                    (forall id id1. mem_id id (ops_of lca) /\ mem_id id1 (diff (snoc (ops_of s1) last1) (ops_of lca)) ==> lt id id1) /\
+                    S.subset (fst (v_of lca)) (fst (do (v_of s1) last1)) /\
+                    S.subset (snd (v_of lca)) (snd (do (v_of s1) last1)))
+          (ensures S.subset (fst (v_of lca)) (fst (v_of s1)) /\
+                   S.subset (snd (v_of lca)) (snd (v_of s1))) =
+  split_prefix init_st (ops_of lca) (ops_of s1);
+  lem_foldl (v_of lca) (diff (ops_of s1) (ops_of lca))
+
+#push-options "--z3rlimit 300" 
+let check (lca s1 s2:st) (last1 last2:op_t)
+  : Lemma (requires do_pre (v_of s1) last1 /\ do_pre (v_of s2) last2 /\ 
+                    consistent_branches lca (do_st s1 last1) (do_st s2 last2) /\
+                    consistent_branches lca s1 s2 /\
+                    fst last1 <> fst last2 /\
+                    merge_pre (v_of lca) (do (v_of s1) last1) (do (v_of s2) last2) /\
+                    //merge_pre (v_of lca) (do (v_of s1) last1) (v_of s2) /\
+                    merge_pre (v_of lca) (v_of s1) (do (v_of s2) last2))
+          (ensures (Add_after? (snd last1) /\ Add_after? (snd last2) ==>
+                      fst last1 <> get_after_id last2 (*/\ fst last2 <> get_after_id last1*))) = ()//(Remove? (snd last1) /\ Add_after? (snd last2) ==> fst last2 <> get_rem_id last1)) = ()
+
+let check' (lca s1 s2:st) (last1 last2:op_t)
+  : Lemma (requires do_pre (v_of s1) last1 /\ do_pre (v_of s2) last2 /\ 
+                    consistent_branches lca (do_st s1 last1) (do_st s2 last2) /\
+                    consistent_branches lca s1 s2 /\
+                    fst last1 <> fst last2 /\
+                    merge_pre (v_of lca) (do (v_of s1) last1) (do (v_of s2) last2) /\
+                    merge_pre (v_of lca) (do (v_of s1) last1) (v_of s2))
+          (ensures (Add_after? (snd last1) /\ Add_after? (snd last2) ==>
+                      fst last2 <> get_after_id last1)) = 
+  check lca s2 s1 last2 last1
+
+let check'' (lca s1 s2:st) (last1 last2:op_t)
+  : Lemma (requires do_pre (v_of s1) last1 /\ do_pre (v_of s2) last2 /\ 
+                    consistent_branches lca (do_st s1 last1) (do_st s2 last2) /\
+                    consistent_branches lca s1 s2 /\
+                    fst last1 <> fst last2 /\
+                    merge_pre (v_of lca) (do (v_of s1) last1) (do (v_of s2) last2) /\
+                    //merge_pre (v_of lca) (do (v_of s1) last1) (v_of s2) /\
+                    merge_pre (v_of lca) (v_of s1) (do (v_of s2) last2))
+          (ensures (Add_after? (snd last1) /\ Add_after? (snd last2) ==>
+                      fst last2 <> get_after_id last1)) = ()
+                      
+let check1 (lca s1 s2:st) (last1 last2:op_t)
+  : Lemma (requires do_pre (v_of s1) last1 /\ do_pre (v_of s2) last2 /\ 
+                    consistent_branches lca (do_st s1 last1) (do_st s2 last2) /\
+                    consistent_branches lca s1 s2 /\
+                    fst last1 <> fst last2 /\
+                    merge_pre (v_of lca) (do (v_of s1) last1) (do (v_of s2) last2) /\
+                    merge_pre (v_of lca) (v_of s1) (do (v_of s2) last2))
+          (ensures (Remove? (snd last2) /\ Add_after? (snd last1) ==> fst last1 <> get_rem_id last2)) = ()
+                      
 let rec invalid_exec (lca s1 s2:st) (last1 last2:op_t)
   : Lemma (requires do_pre (v_of s1) last1 /\ do_pre (v_of s2) last2 /\ 
                     consistent_branches lca (do_st s1 last1) (do_st s2 last2) /\
@@ -245,21 +447,26 @@ let rec invalid_exec (lca s1 s2:st) (last1 last2:op_t)
 let linearizable_gt0_s1' (lca s1 s2:st) (last1 last2:op_t)
   : Lemma (requires do_pre (v_of s1) last1 /\ do_pre (v_of s2) last2 /\ 
                     consistent_branches lca (do_st s1 last1) (do_st s2 last2) /\
-                    consistent_branches lca s1 (do_st s2 last2) /\
+                    //consistent_branches lca s1 (do_st s2 last2) /\
                     consistent_branches lca s1 s2 /\
-                    is_prefix (ops_of lca) (ops_of s2) /\
+                    //is_prefix (ops_of lca) (ops_of s2) /\
                     fst last1 <> fst last2 /\
-                    First_then_second? (resolve_conflict last1 last2) /\
+                    //First_then_second? (resolve_conflict last1 last2) /\
                     //Remove? (snd last1) /\ Remove? (snd last2) /\ //all done
-                    //Add_after? (snd last1) /\ Remove? (snd last2) /\
+                    Add_after? (snd last1) /\ Remove? (snd last2) /\
                     //Add_after? (snd last1) /\ Add_after? (snd last2) /\ get_after_id last1 <> get_after_id last2 /\
                     //Add_after? (snd last1) /\ Add_after? (snd last2) /\ get_after_id last1 = get_after_id last2 /\ fst last1 > fst last2 /\
-                    merge_pre (v_of lca) (do (v_of s1) last1) (do (v_of s2) last2))
-          (ensures merge_pre (v_of lca) (v_of s1) (do (v_of s2) last2) /\ //only w/o subset pre
-                   do_pre (concrete_merge (v_of lca) (v_of s1) (do (v_of s2) last2)) last1 /\ //only with subset pre
+                    merge_pre (v_of lca) (do (v_of s1) last1) (do (v_of s2) last2) /\
+                    merge_pre (v_of lca) (v_of s1) (do (v_of s2) last2))
+          (ensures //merge_pre (v_of lca) (v_of s1) (do (v_of s2) last2) /\ //only w/o subset pre
+                   do_pre (concrete_merge (v_of lca) (v_of s1) (do (v_of s2) last2)) last1 (*/\ //only with subset pre
                    eq (do (concrete_merge (v_of lca) (v_of s1) (do (v_of s2) last2)) last1)
-                      (concrete_merge (v_of lca) (do (v_of s1) last1) (do (v_of s2) last2))) = 
+                      (concrete_merge (v_of lca) (do (v_of s1) last1) (do (v_of s2) last2)*)) = 
   invalid_exec lca s1 s2 last1 last2
+  (*assert ((Remove? (snd last2) /\ Add_after? (snd last1) ==> fst last1 <> get_rem_id last2) /\
+          (Add_after? (snd last1) /\ Add_after? (snd last2) ==>
+                      fst last1 <> get_after_id last2 /\ fst last2 <> get_after_id last1));*)
+  ()
 
 let linearizable_gt0_s2' (lca s1 s2:st) (last1 last2:op_t)
   : Lemma (requires do_pre (v_of s1) last1 /\ do_pre (v_of s2) last2 /\ 
@@ -282,4 +489,4 @@ let linearizable_gt0_s2' (lca s1 s2:st) (last1 last2:op_t)
   assert ((Remove? (snd last1) /\ Add_after? (snd last2) ==> fst last2 <> get_rem_id last1) /\
           (Add_after? (snd last1) /\ Add_after? (snd last2) ==>
                       fst last1 <> get_after_id last2 /\ fst last2 <> get_after_id last1));
-  ()
+  ()*)
